FStar.Algebra.Setoid.fst
@@ -1,0 +1,88 @@
+module FStar.Algebra.Setoid
+
+module TC = FStar.Tactics.Typeclasses
+module P = FStar.PropositionalExtensionality
+
+open FStar.Tactics
+
+class equivalence_relation a = {
+  eq : a -> a -> bool;
+  reflexivity : (x:a -> Lemma (eq x x));
+  symmetry: (x:a -> y:a -> Lemma (x `eq` y <==> y `eq` x));
+  transitivity: (x:a -> y:a -> z:a -> Lemma (((eq x y) /\ (eq y z)) ==> eq x z));  
+} 
+
+type indicator a = a -> bool
+
+private let eqclass_indicator #a {| equivalence_relation a |} (x:a) (y:a) = eq x y
+
+let make_eqclass #a {| equivalence_relation a |} (sample:a) : indicator a = eqclass_indicator sample
+
+let (!) #a {| equivalence_relation a |} x : indicator a = make_eqclass x
+
+class has_mul t {| equivalence_relation t |} = {
+  mul: t -> t -> t;
+  congruence: (x:t) -> (y:t) -> (z:t) -> (w:t) 
+    -> Lemma (requires eq x z /\ eq y w) (ensures eq (mul x y) (mul z w))  
+}
+
+let ec_eq #t {| equivalence_relation t |} #x (f: indicator t{f == !x}) #y (g: indicator t{g == !y})
+  = eq x y
+
+let try_compare #a {| equivalence_relation a |} (x y:a) (op: a->a->a) = 
+  ec_eq !x !y
+
+
+let is_reflexive #a (f: bool_func a) = forall (x:a). f a a
+
+type setoid #a {| equivalence_relation a |} (x:a) = z:a{eq z x}
+
+let ( ! ) #a {| eq: equivalence_relation a |} (x:a) = setoid x
+ 
+noeq type magma a {| equivalence_relation a |} = {
+  op: a -> a -> a;
+  congruence: (x:a) -> (y:a) -> (z:a) -> (w: a) 
+    -> Lemma (requires eq x z /\ eq y w) (ensures eq (op x y) (op z w))
+}
+ 
+
+let op #a {| equivalence_relation a |} (m: magma a) (#x #y: a) (p:Type{p == !x}) (q:Type{q == !y})
+  = !(m.op x y) 
+
+let op_congruence #a {| equivalence_relation a |} 
+  (m: magma a) 
+  (x y:a) 
+  : Lemma (ensures !(x `m.op` y) == op m !x !y ) = ()
+ 
+
+open FStar.Tactics
+
+let prop_ext #a (p q:a -> prop) (v:a)
+  : Lemma (requires (forall x. p x <==> q x))
+          (ensures p v == q v)
+  = P.apply (p v) (q v)
+
+let refinement_equality (a:Type) (p q:a -> prop)
+  : Lemma
+    (requires forall x. p x <==> q x)
+    (ensures (x:a { p x } == x:a { q x }))
+  = assert (x:a { p x } == x:a { q x })
+        by (pointwise
+             (fun _ ->
+               try mapply (quote (prop_ext #a p q))
+               with _ -> trefl());
+            trefl())
+
+let eq_lemma #a {| equivalence_relation a |} (x y: a)
+  : Lemma (requires eq x y) (ensures !x == !y) = 
+  let equality (z:a) : Lemma (eq z x == eq z y) = 
+      transitivity z x y;
+      symmetry y x;
+      transitivity z y x in
+  Classical.forall_intro equality;
+  let f1 (p:a) : prop = eq p x == true in
+  let f2 (p:a) : prop = eq p y == true in  
+  assert_norm (setoid x == z:a{f1 z});
+  assert_norm (setoid y == z:a{f2 z});
+  refinement_equality a f1 f2 
+  
